bedrock2/src/bedrock2/anyval.v
@@ -1,0 +1,12 @@
+Require Import bedrock2.Lift1Prop.
+
+Definition anyval{word mem T: Type}(p: T -> word -> mem -> Prop)(a: word): mem -> Prop :=
+  ex1 (fun v => p v a).
+
+(* makes __ a keyword, so "let __ := uselessvalue in blah" in Ltac
+   doesn't parse any more!
+Notation "p '__' a" := (anyval p a) (at level 20, a at level 9).
+Infix "__" := anyval (at level 20).
+*)
+
+Notation "p ? a" := (anyval p a) (at level 20, a at level 9).
